# Introduction to Optimization  
**Final exam solutions, 22.10.2015**

### 1. 

The gradient and the Hessian matrix for \( f(x) = e^{-x_1-x_2} + x_1^2 + x_2^2 \) are

$$
\nabla f(x) = \begin{bmatrix} 2x_1 - e^{-x_1-x_2} \\ 2x_2 - e^{-x_1-x_2} \end{bmatrix},
\quad
H_f = \begin{bmatrix} 2 + e^{-x_1-x_2} & e^{-x_1-x_2} \\ e^{-x_1-x_2} & 2 + e^{-x_1-x_2} \end{bmatrix}.
$$

The Hessian matrix is positive definite for every \( x \in \mathbb{R}^2 \) (determinant = 4 + 3e^{-x_1-x_2} > 0 and trace > 0), and therefore \( f \) is strictly convex. The Newton iterations are
$$
x^{(k+1)} = x^{(k)} - \left[ H_f(x^{(k)} \right]^{-1} \nabla f(x^{(k)}).

Starting point \( x^{(0)} = \begin{bmatrix} 0 \\ 0 \end{bmatrix}. Next iteration is
$$
x^{(1)} = \begin{bmatrix} 1/4 \\ 1/4 \end{bmatrix} \quad \text{and} \quad \nabla f(x^{(1)}) \approx \begin{bmatrix} -0.1065 \\ -0.1065 \end{bmatrix}.
$$

Moreover,
$$
x^{(2)} \approx \begin{bmatrix} 0.2832 \\ 0.2832 \end{bmatrix} \quad \text{and} \quad \nabla f(x^{(2)}) \approx \begin{bmatrix} -0.0013 \\ -0.0013 \end{bmatrix}.

### 2. The function is quadratic since
$$
f(x) = \frac{1}{2} x^{\top} A x - b^{\top} x \quad \text{with} \quad A = \begin{bmatrix} 8 & -2 \\ -2 & 4 \end{bmatrix}, \quad b^{\top} = [-2 \quad -3].

Starting the conjugate gradient method from the initial point x^{(0)} = 0 \end{pmatrix} 0 \end{bmatrix}, we obtain r^{(0)} = d_0 = \begin{bmatrix} -2 \\ -3 \end{bmatrix},

β_0 = 0, α_0 = 13/44 and
$$
x^{(1)} = \frac{13}{44} \begin{bmatrix} -2 \\ -3 \end{bmatrix} \quad \text{and} \quad r^{(1)} = \frac{7}{22} \begin{bmatrix} 3 \\ -2 \end{bmatrix}.

Next, β_1 = \frac{72}{222}, d_1 = \frac{7 \cdot 7\cdot13}{222} \begin{bmatrix} 4 \\ -5 \end{bmatrix}, α_1 = \frac{11}{7\cdot13} and
$$
x^{(2)} = \begin{bmatrix} -1/2 \\ -1 \end{bmatrix} \quad \text{and} \quad r^{(2)} = \begin{bmatrix} 0 \\ 0 \end{bmatrix}.
$$

Thus, x^{(2)} is the optimal solution.

### 3. From the KKT-conditions we obtain
$$
\begin{align*}
e^{x1-x2} + u_1 e^{x1} - u_2 &= 0, \\
-e^{x1-x2} + u_1 e^{x2} &= 0, \\
u_1 (e^{x1} + e^{x2} -20) &= 0, \\
u_2 x_1 &= 0, \\
u_1, u_2 &\geq 0.
\end{align*}
$$

The conditions are satisfied when u_1 \neq 0 \text{ and } u_2 \neq 0 (all other possibilities lead to contradiction). Since u_2 \neq 0, we must have x_1 = 0 \text{ and } e^{x1} + e^{x2} -20 = 0. Thus, e^{x2} = 19 \text{ and therefore } x_2 = \ln 19. Moreover,
u_1 = \frac{1}{361} \text{ and } u_2 = \frac{20}{361}.

### 4. The Lagrangian is
$$
L(x,u) = x_1^2 + x_1 x_2 + x_2^2 -x_1 -x_2 + u_1(x_1 -1) + u_2(-x_1 -1) + u_3(x_2 -1) + u_4(-x_2 -1).
$$

The gradient is
$$
\nabla L(x,u) = \begin{bmatrix} 2x_1 + x_2 -1 + u_1 - u_2 \\ x_1 + 2x_2 -1 + u_3 -u_4 \end{bmatrix}
$$

and setting the gradient to zero and solving x_1 = \frac{1}{3}(1 -2u_1 + 2u_2 + u_3 -u_4), x_2 = \frac{1}{3}(1 + u_1 -u_2 -2u_3 + 2u_4).

Substituting these to the Lagrangian we obtain the dual function
G(u) = - (1/3)u_3^2 + (2/3)u_3 u_4 + (1/3)u_3 u_1 - (1/3)u_3 u_2 - (1/3)u_4^2 - (1/3)u_4 u_1 + (1/3)u_4 u_2 - (1/3)u_1^2 + (2/3)u_1 u_2 - (1/3)u_2^2 -1/3 - (2/3)u_3 - (2/3)u_1 - (4/3)u_4 - (4/3)u_ YEARS.

The roots of the gradient of the dual function do not exist, and therefore the global solution x_opt = \begin{bmatrix} 1/3 \\ 1/3 \end{bmatrix}^T is the solution.